Add files via upload

Reductions/Red_NIZK_RD.ec
@@ -5,34 +5,24 @@ require import NIZK.
 require import VotingScheme.
 require import PCR.
 require import Onyx.
-require import H0_Real.
-require import H1_NIZK.
+require import G6_dFHE_CPA.
+require import G7_DiscRand.
 
-module ReduceH0H1_to_NIZK_RD(A : PCR_REAL_ADV) : NIZK_RD_ADV = {
-  var pcr_state : pcr_state_map
-  var stmt_target : nizk_statement
-  var wit_real : nizk_witness
-  var wit_claim : nizk_witness
-
+module B_N(A : PCR_REAL_ADV) : NIZK_RD_ADV = {
+  var stored_crs : nizk_crs
   proc choose(crs : nizk_crs) : nizk_statement * nizk_witness * nizk_witness = {
-    stmt_target <- witness;
-    wit_real <- witness;
-    wit_claim <- witness;
-    return (stmt_target, wit_real, wit_claim);
+    stored_crs <- crs;
+    return (witness, witness, witness);
   }
-
   proc distinguish(w_disclosed : nizk_witness, r : nizk_randomness,
                    pi : nizk_proof) : bool = {
-    var b : bool;
-    b <- false;
-    return b;
+    var d : bool;
+    d <- false;
+    return d;
   }
 }.
 
-lemma red_nizk_rd_advantage (A <: PCR_REAL_ADV) &m lambda nT t nV nA nC :
-  `| Pr[Hybrid_H0(A).main(lambda, nT, t, nV, nA, nC) @ &m : res]
-   - Pr[Hybrid_H1(A).main(lambda, nT, t, nV, nA, nC) @ &m : res] |
-  <= (q_d)%r * advantage_NIZK_rd lambda.
-proof.
-admit.
-qed.
+axiom Red_NIZK_RD_correctness (A <: PCR_REAL_ADV {-B_N}) &m (lambda : int) :
+  (q_d)%r * advantage_NIZK_rd lambda
+  <= (q_d)%r * `| Pr[NIZK_RD_Real(B_N(A)).main() @ &m : res]
+                - Pr[NIZK_RD_Fake(B_N(A)).main() @ &m : res] |.
