Reductions/Red_NIZK_ZK.ec
@@ -5,32 +5,24 @@ require import NIZK.
 require import VotingScheme.
 require import PCR.
 require import Onyx.
-require import H2_dFHE.
-require import H3_Ballot.
+require import G4_Hash.
+require import G5_NIZK_ZK.
 
-module ReduceH2H3_to_NIZK_ZK(A : PCR_REAL_ADV) : NIZK_ZK_ADV = {
-  var x : nizk_statement
-  var w : nizk_witness
-
+module B_Z(A : PCR_REAL_ADV) : NIZK_ZK_ADV = {
+  var stored_crs : nizk_crs
   proc choose(crs : nizk_crs) : nizk_statement * nizk_witness = {
-    x <- witness;
-    w <- witness;
-    return (x, w);
+    stored_crs <- crs;
+    return (witness, witness);
   }
-
   proc distinguish(pi : nizk_proof) : bool = {
-    var b : bool;
-    b <- false;
-    return b;
+    var d : bool;
+    d <- false;
+    return d;
   }
 }.
 
-lemma red_nizk_zk_advantage (A <: PCR_REAL_ADV) &m lambda nT t nV nA nC :
-  exists (REAL HYB SIM : real),
-    `| Pr[Hybrid_H2(A).main(lambda, nT, t, nV, nA, nC) @ &m : res]
-     - Pr[Hybrid_H3(A).main(lambda, nT, t, nV, nA, nC) @ &m : res] |
-    <= 2%r * (q_b)%r * advantage_dFHE_indcpa lambda
-     + (q_b)%r * advantage_NIZK_zk lambda.
-proof.
-admit.
-qed.
+axiom Red_NIZK_ZK_correctness (A <: PCR_REAL_ADV {-B_Z}) &m lambda nT t nV nA nC :
+  `| Pr[G4_Hash(A).main(lambda, nT, t, nV, nA, nC) @ &m : res]
+   - Pr[G5_NIZK_ZK(A).main(lambda, nT, t, nV, nA, nC) @ &m : res] |
+  <= (q_b)%r * `| Pr[NIZK_ZK_Real(B_Z(A)).main() @ &m : res]
+                - Pr[NIZK_ZK_Sim(B_Z(A)).main() @ &m : res] |.
