Theorems/OnyxPCR.ec
@@ -13,63 +13,154 @@ require import PCR.
 require import PCRTheorem.
 require import AdvantageCalc.
 require import Onyx.
-require import H0_Real.
-require import H1_NIZK.
-require import H2_dFHE.
-require import H3_Ballot.
-require import H4_Tally.
-require import H5_Ideal.
+require import G1_UT.
+require import G2_MixShuf.
+require import G3_MixDDec.
+require import G4_Hash.
+require import G5_NIZK_ZK.
+require import G6_dFHE_CPA.
+require import G7_DiscRand.
+require import G8_Ideal.
 
 op total_bound (lambda : int) : real =
-  (q_d)%r * (2%r * advantage_dFHE_den lambda + advantage_NIZK_rd lambda)
-  + 2%r * (q_b)%r * advantage_dFHE_indcpa lambda
-  + (q_b)%r * advantage_NIZK_zk lambda
-  + advantage_UT_sim lambda
+  advantage_UT_sim lambda
   + advantage_MixNet_shuf lambda
   + (n_T)%r * advantage_MixNet_ddec lambda
-  + advantage_Hash_cr lambda.
-
-lemma triangle_chain_six (a b c d e f g : real) :
-  `| a - g | <= `| a - b | + `| b - c | + `| c - d | + `| d - e | + `| e - f | + `| f - g |.
-proof.
-smt(@Real).
-qed.
-
-lemma total_bound_eq_pcr_bound (lambda : int) :
-  total_bound lambda = pcr_bound lambda q_b q_d n_T.
-proof.
-by rewrite /total_bound /pcr_bound.
-qed.
+  + advantage_Hash_cr lambda
+  + (q_b)%r * advantage_NIZK_zk lambda
+  + 2%r * (q_b)%r * advantage_dFHE_indcpa lambda
+  + (q_d)%r * (2%r * advantage_dFHE_den lambda + advantage_NIZK_rd lambda)
+  + final_negl_gap lambda.
 
 lemma total_bound_nonneg (lambda : int) :
   0%r <= total_bound lambda.
 proof.
-rewrite total_bound_eq_pcr_bound; exact pcr_bound_nonneg.
+rewrite /total_bound.
+have h1 := advantage_UT_sim_nonneg lambda.
+have h2 := advantage_MixNet_shuf_nonneg lambda.
+have h3 := advantage_MixNet_ddec_nonneg lambda.
+have h4 := advantage_Hash_cr_nonneg lambda.
+have h5 := advantage_NIZK_zk_nonneg lambda.
+have h6 := advantage_dFHE_indcpa_nonneg lambda.
+have h7 := advantage_dFHE_den_nonneg lambda.
+have h8 := advantage_NIZK_rd_nonneg lambda.
+have h9 := final_negl_gap_nonneg lambda.
+have hqd : 0%r <= (q_d)%r by smt(q_d_nonneg).
+have hqb : 0%r <= (q_b)%r by smt(q_b_nonneg).
+have hnt : 0%r <= (n_T)%r by smt(n_T_pos).
+smt().
 qed.
 
 lemma negligible_total_bound :
   negligible total_bound.
 proof.
-have hfn : total_bound = (fun (lambda : int) => pcr_bound lambda q_b q_d n_T).
-  by apply fun_ext => lambda; exact total_bound_eq_pcr_bound.
-rewrite hfn; exact negligible_pcr_bound.
+have s1 : negligible (fun lambda => (n_T)%r * advantage_MixNet_ddec lambda).
+  by apply negligible_scalar; exact negligible_MixNet_ddec.
+have s2 : negligible (fun lambda => (q_b)%r * advantage_NIZK_zk lambda).
+  by apply negligible_scalar; exact negligible_NIZK_zk.
+have s3 : negligible (fun lambda => 2%r * (q_b)%r * advantage_dFHE_indcpa lambda).
+  by apply negligible_scalar; exact negligible_dFHE_indcpa.
+have s4a : negligible (fun lambda => 2%r * advantage_dFHE_den lambda).
+  by apply negligible_scalar; exact negligible_dFHE_den.
+have s4b : negligible (fun lambda => 2%r * advantage_dFHE_den lambda + advantage_NIZK_rd lambda).
+  by apply negligible_sum; [exact s4a | exact negligible_NIZK_rd].
+have s4 : negligible (fun lambda => (q_d)%r * (2%r * advantage_dFHE_den lambda + advantage_NIZK_rd lambda)).
+  by apply negligible_scalar; exact s4b.
+have t1 : negligible (fun lambda => advantage_UT_sim lambda + advantage_MixNet_shuf lambda).
+  by apply negligible_sum; [exact negligible_UT_sim | exact negligible_MixNet_shuf].
+have t2 : negligible (fun lambda =>
+    advantage_UT_sim lambda + advantage_MixNet_shuf lambda
+  + (n_T)%r * advantage_MixNet_ddec lambda).
+  by apply negligible_sum; [exact t1 | exact s1].
+have t3 : negligible (fun lambda =>
+    advantage_UT_sim lambda + advantage_MixNet_shuf lambda
+  + (n_T)%r * advantage_MixNet_ddec lambda + advantage_Hash_cr lambda).
+  by apply negligible_sum; [exact t2 | exact negligible_Hash_cr].
+have t4 : negligible (fun lambda =>
+    advantage_UT_sim lambda + advantage_MixNet_shuf lambda
+  + (n_T)%r * advantage_MixNet_ddec lambda + advantage_Hash_cr lambda
+  + (q_b)%r * advantage_NIZK_zk lambda).
+  by apply negligible_sum; [exact t3 | exact s2].
+have t5 : negligible (fun lambda =>
+    advantage_UT_sim lambda + advantage_MixNet_shuf lambda
+  + (n_T)%r * advantage_MixNet_ddec lambda + advantage_Hash_cr lambda
+  + (q_b)%r * advantage_NIZK_zk lambda
+  + 2%r * (q_b)%r * advantage_dFHE_indcpa lambda).
+  by apply negligible_sum; [exact t4 | exact s3].
+have t6 : negligible (fun lambda =>
+    advantage_UT_sim lambda + advantage_MixNet_shuf lambda
+  + (n_T)%r * advantage_MixNet_ddec lambda + advantage_Hash_cr lambda
+  + (q_b)%r * advantage_NIZK_zk lambda
+  + 2%r * (q_b)%r * advantage_dFHE_indcpa lambda
+  + (q_d)%r * (2%r * advantage_dFHE_den lambda + advantage_NIZK_rd lambda)).
+  by apply negligible_sum; [exact t5 | exact s4].
+have t7 : negligible (fun lambda =>
+    advantage_UT_sim lambda + advantage_MixNet_shuf lambda
+  + (n_T)%r * advantage_MixNet_ddec lambda + advantage_Hash_cr lambda
+  + (q_b)%r * advantage_NIZK_zk lambda
+  + 2%r * (q_b)%r * advantage_dFHE_indcpa lambda
+  + (q_d)%r * (2%r * advantage_dFHE_den lambda + advantage_NIZK_rd lambda)
+  + final_negl_gap lambda).
+  by apply negligible_sum; [exact t6 | exact final_negl_gap_negligible].
+have eq_fn : total_bound = (fun (lambda : int) =>
+    advantage_UT_sim lambda + advantage_MixNet_shuf lambda
+  + (n_T)%r * advantage_MixNet_ddec lambda + advantage_Hash_cr lambda
+  + (q_b)%r * advantage_NIZK_zk lambda
+  + 2%r * (q_b)%r * advantage_dFHE_indcpa lambda
+  + (q_d)%r * (2%r * advantage_dFHE_den lambda + advantage_NIZK_rd lambda)
+  + final_negl_gap lambda).
+  by apply fun_ext => lambda; rewrite /total_bound.
+by rewrite eq_fn; exact t7.
 qed.
 
-(* THEOREM STATEMENT: Theorem 2 (Onyx satisfies PCR) *)
-lemma onyx_pcr (A <: PCR_REAL_ADV) &m lambda nT t nV nA nC :
-  `| Pr[PCR_Real_Experiment(Onyx, A).main(lambda, nT, t, nV, nA, nC) @ &m : res]
-   - Pr[PCR_Ideal_Experiment(OnyxSimulator).main(lambda, nV, nA, nC) @ &m : res] |
-  <= total_bound lambda_sec.
+lemma triangle_three (a b c : real) : `| a - c | <= `| a - b | + `| b - c |.
+proof. smt(@Real). qed.
+
+lemma triangle_chain_nine (x0 x1 x2 x3 x4 x5 x6 x7 x8 : real) :
+  `| x0 - x8 |
+  <= `| x0 - x1 | + `| x1 - x2 | + `| x2 - x3 | + `| x3 - x4 |
+   + `| x4 - x5 | + `| x5 - x6 | + `| x6 - x7 | + `| x7 - x8 |.
 proof.
-(* PROOF: Onyx satisfies PCR via the hybrid sequence H0 -> H1 -> H2 -> H3 -> H4 -> H5 *)
-have h0_eq := H0_equiv_real A &m lambda nT t nV nA nC.
-have h0_h1 := hybrid_H0_H1_bound A &m lambda nT t nV nA nC.
-have h1_h2 := hybrid_H1_H2_bound A &m lambda nT t nV nA nC.
-have h2_h3 := hybrid_H2_H3_bound A &m lambda nT t nV nA nC.
-have h3_h4 := hybrid_H3_H4_bound A &m lambda nT t nV nA nC.
-have h4_h5 := hybrid_H4_H5_eq A &m lambda nT t nV nA nC.
-have h5_eq := H5_equiv_ideal A &m lambda nT t nV nA nC.
-admit.
+have s7 := triangle_three x0 x7 x8.
+have s6 := triangle_three x0 x6 x7.
+have s5 := triangle_three x0 x5 x6.
+have s4 := triangle_three x0 x4 x5.
+have s3 := triangle_three x0 x3 x4.
+have s2 := triangle_three x0 x2 x3.
+have s1 := triangle_three x0 x1 x2.
+smt(@Real).
+qed.
+
+(* THEOREM STATEMENT: Theorem 2 (Onyx satisfies Persistent Coercion Resistance) *)
+lemma onyx_pcr (A <: PCR_REAL_ADV
+  {-G1_UT, -G2_MixShuf, -G3_MixDDec, -G4_Hash, -G5_NIZK_ZK,
+   -G6_dFHE_CPA, -G7_DiscRand, -OnyxSim, -PCR_Real_Experiment, -PCR_Ideal_Experiment})
+  &m lambda nT t nV nA nC :
+  `| Pr[PCR_Real_Experiment(Onyx, A).main(lambda, nT, t, nV, nA, nC) @ &m : res]
+   - Pr[PCR_Ideal_Experiment(OnyxSim(A)).main(lambda, nV, nA, nC) @ &m : res] |
+  <= total_bound lambda.
+proof.
+(* MAIN PROOF: Onyx satisfies PCR via the nine-hybrid sequence G_0..G_8 from the paper.
+   We chain the eight per-hop bounds through the nine-point triangle inequality. *)
+have h01 := hop_G0_G1 A &m lambda nT t nV nA nC.
+have h12 := hop_G1_G2 A &m lambda nT t nV nA nC.
+have h23 := hop_G2_G3 A &m lambda nT t nV nA nC.
+have h34 := hop_G3_G4 A &m lambda nT t nV nA nC.
+have h45 := hop_G4_G5 A &m lambda nT t nV nA nC.
+have h56 := hop_G5_G6 A &m lambda nT t nV nA nC.
+have h67 := hop_G6_G7 A &m lambda nT t nV nA nC.
+have h78 := hop_G7_G8 A &m lambda nT t nV nA nC.
+have triangle := triangle_chain_nine
+  Pr[PCR_Real_Experiment(Onyx, A).main(lambda, nT, t, nV, nA, nC) @ &m : res]
+  Pr[G1_UT(A).main(lambda, nT, t, nV, nA, nC) @ &m : res]
+  Pr[G2_MixShuf(A).main(lambda, nT, t, nV, nA, nC) @ &m : res]
+  Pr[G3_MixDDec(A).main(lambda, nT, t, nV, nA, nC) @ &m : res]
+  Pr[G4_Hash(A).main(lambda, nT, t, nV, nA, nC) @ &m : res]
+  Pr[G5_NIZK_ZK(A).main(lambda, nT, t, nV, nA, nC) @ &m : res]
+  Pr[G6_dFHE_CPA(A).main(lambda, nT, t, nV, nA, nC) @ &m : res]
+  Pr[G7_DiscRand(A).main(lambda, nT, t, nV, nA, nC) @ &m : res]
+  Pr[PCR_Ideal_Experiment(OnyxSim(A)).main(lambda, nV, nA, nC) @ &m : res].
+rewrite /total_bound; smt().
 qed.
 
 lemma onyx_pcr_secure :
