Hybrids/G6_dFHE_CPA.ec
@@ -1,0 +1,121 @@
+require import AllCore Distr Real List FSet FMap Bool DBool.
+require import Preamble.
+require import Negligible.
+require import DFHE.
+require import NIZK.
+require import UT.
+require import MixNet.
+require import Hash.
+require import VotingScheme.
+require import Policy.
+require import PCR.
+require import Onyx.
+require import G5_NIZK_ZK.
+
+op canonical_vote : vote.
+op canonical_cred : credential.
+
+axiom canonical_vote_valid : valid_vote_index canonical_vote.
+
+module G6_dFHE_CPA(A : PCR_REAL_ADV) = {
+  var bb : election_bb
+  var st : pcr_state_map
+  var disc : int fset
+  var beta_bit : bool
+  var pk_v : election_pk
+  var shares_v : (election_sk_share * election_hint_t) list
+  var creds : election_credential list
+  var reg_R : election_register_record
+  var corrupt_D : int fset
+  var coerce_H : int fset
+  var alphas : (int, int) fmap
+  var ut_sim_pp : ut_pp
+  var ut_sim_shares : ut_share list
+  var mix_sim_pp : mixnet_pp
+  var mix_sim_pf : mixnet_proof
+  var ddec_sim_parts : (mixnet_partial list * mixnet_ddec) list
+  var shadow_record : behavior_list
+
+  proc cast_canonical_ballot(c : election_credential, v : vote) : election_ballot = {
+    var rv_can, rc_can : randomness;
+    var cv_ct, cc_ct : ciphertext;
+    var stmt : nizk_statement;
+    var pi_sim : nizk_proof;
+    rv_can <- witness;
+    rc_can <- witness;
+    cv_ct <- dFHE_enc witness canonical_vote rv_can;
+    cc_ct <- dFHE_enc witness (credential_to_int canonical_cred) rc_can;
+    stmt <- (cv_ct, cc_ct, witness);
+    pi_sim <$ nizk_simulate witness stmt;
+    return (cv_ct, cc_ct, pi_sim);
+  }
+
+  proc main(lambda nT t nV nA nC : int) : bool = {
+    var d : bool;
+    var msgs : bb_message list;
+    var valid_msgs : ballot list;
+    var ballot_seq : behavior_list;
+    var i : int;
+    var v : vote;
+    var b_cur : election_ballot;
+    var r_result : election_result;
+    var pi_result : election_tally_proof;
+    var gated : bool;
+    var b_post : bool;
+    var dummy_cts : mixnet_ciphertext list;
+    var dummy_mixed : mixnet_ciphertext list;
+    var dummy_sks : mixnet_skey list;
+    var dummy_plaintexts : int list;
+
+    bb <- [];
+    st <- empty;
+    disc <- fset0;
+    shadow_record <- [];
+    (ut_sim_pp, ut_sim_shares) <$ ut_sim_setup lambda nT t;
+    dummy_cts <- [];
+    dummy_mixed <- [];
+    dummy_sks <- [];
+    dummy_plaintexts <- [];
+    mix_sim_pp <- witness;
+    mix_sim_pf <$ mixnet_sim_mix mix_sim_pp dummy_cts dummy_mixed;
+    ddec_sim_parts <$ mixnet_sim_ddec mix_sim_pp dummy_sks dummy_cts dummy_plaintexts;
+    (pk_v, shares_v) <@ Onyx.setup(lambda, nT, t);
+    (creds, reg_R) <@ Onyx.register(lambda, pk_v, nV);
+    corrupt_D <@ A.corrupt(reg_R);
+    (coerce_H, alphas) <@ A.coerce_choose(creds);
+    ballot_seq <- [];
+    beta_bit <$ {0,1};
+    ballot_seq <- coerce_adjust ballot_seq coerce_H alphas beta_bit;
+    i <- 0;
+    d <- false;
+    while (i < size ballot_seq) {
+      msgs <@ A.board_phase(bb);
+      valid_msgs <- extract_valid_ballots pk_v msgs bb;
+      bb <- bb ++ valid_msgs;
+      v <- snd (nth witness ballot_seq i);
+      b_cur <@ cast_canonical_ballot(nth witness creds (fst (nth witness ballot_seq i) - 1), v);
+      bb <- bb ++ [b_cur];
+      shadow_record <- shadow_record ++ [nth witness ballot_seq i];
+      i <- i + 1;
+    }
+    msgs <@ A.final_post(bb);
+    valid_msgs <- extract_valid_ballots pk_v msgs bb;
+    bb <- bb ++ valid_msgs;
+    r_result <- result_func shadow_record;
+    pi_result <- witness;
+    A.post_tally(r_result, pi_result);
+    gated <- coerce_H \subset disc;
+    if (! gated) {
+      b_post <$ {0,1};
+      d <- b_post;
+    } else {
+      d <@ A.final_guess();
+    }
+    return d;
+  }
+}.
+
+axiom hop_G5_G6 (A <: PCR_REAL_ADV {-G5_NIZK_ZK, -G6_dFHE_CPA}) &m lambda nT t nV nA nC :
+  `| Pr[G5_NIZK_ZK(A).main(lambda, nT, t, nV, nA, nC) @ &m : res]
+   - Pr[G6_dFHE_CPA(A).main(lambda, nT, t, nV, nA, nC) @ &m : res] |
+  <= 2%r * (q_b)%r * advantage_dFHE_indcpa lambda.
