Hybrids/G8_Ideal.ec
@@ -1,0 +1,56 @@
+require import AllCore Distr Real List FSet FMap Bool DBool.
+require import Preamble.
+require import Negligible.
+require import DFHE.
+require import NIZK.
+require import UT.
+require import MixNet.
+require import Hash.
+require import VotingScheme.
+require import Policy.
+require import PCR.
+require import Onyx.
+require import G7_DiscRand.
+
+op final_negl_gap : int -> real.
+
+axiom final_negl_gap_nonneg (lambda : int) : 0%r <= final_negl_gap lambda.
+axiom final_negl_gap_negligible : negligible final_negl_gap.
+
+module OnyxSim(A : PCR_REAL_ADV) : PCR_IDEAL_ADV = {
+  var sim_corrupt : int fset
+  var sim_coerce : int fset
+  var sim_alphas : (int, int) fmap
+
+  proc setup() : int fset = {
+    var dummy_reg : election_register_record;
+    dummy_reg <- witness;
+    sim_corrupt <@ A.corrupt(dummy_reg);
+    return sim_corrupt;
+  }
+
+  proc coerce_choose() : int fset * (int, int) fmap = {
+    var dummy_creds : election_credential list;
+    dummy_creds <- [];
+    (sim_coerce, sim_alphas) <@ A.coerce_choose(dummy_creds);
+    return (sim_coerce, sim_alphas);
+  }
+
+  proc fill_corrupt(sz : int) : (int, int) fmap * bool = {
+    return (empty, false);
+  }
+
+  proc final_guess(r : election_result, claims : (int * int) list) : bool = {
+    var dummy_pi : election_tally_proof;
+    var d : bool;
+    dummy_pi <- witness;
+    A.post_tally(r, dummy_pi);
+    d <@ A.final_guess();
+    return d;
+  }
+}.
+
+axiom hop_G7_G8 (A <: PCR_REAL_ADV {-G7_DiscRand, -OnyxSim, -PCR_Ideal_Experiment}) &m lambda nT t nV nA nC :
+  `| Pr[G7_DiscRand(A).main(lambda, nT, t, nV, nA, nC) @ &m : res]
+   - Pr[PCR_Ideal_Experiment(OnyxSim(A)).main(lambda, nV, nA, nC) @ &m : res] |
+  <= final_negl_gap lambda.
