Reductions/Red_Hash.ec
@@ -1,0 +1,22 @@
+require import AllCore Distr Real List FSet FMap Bool.
+require import Preamble.
+require import Negligible.
+require import Hash.
+require import VotingScheme.
+require import PCR.
+require import Onyx.
+require import G3_MixDDec.
+require import G4_Hash.
+
+module B_H(A : PCR_REAL_ADV) : HASH_CR_ADV = {
+  var stored_chal_pairs : (hash_input * hash_input) list
+  proc find_collision() : hash_input * hash_input = {
+    stored_chal_pairs <- [];
+    return ([], []);
+  }
+}.
+
+axiom Red_Hash_correctness (A <: PCR_REAL_ADV {-B_H}) &m lambda nT t nV nA nC :
+  `| Pr[G3_MixDDec(A).main(lambda, nT, t, nV, nA, nC) @ &m : res]
+   - Pr[G4_Hash(A).main(lambda, nT, t, nV, nA, nC) @ &m : res] |
+  <= Pr[Hash_CR_Game(B_H(A)).main() @ &m : res].
