Reductions/Red_MixDDec.ec
@@ -1,0 +1,31 @@
+require import AllCore Distr Real List FSet FMap Bool.
+require import Preamble.
+require import Negligible.
+require import MixNet.
+require import VotingScheme.
+require import PCR.
+require import Onyx.
+require import G2_MixShuf.
+require import G3_MixDDec.
+
+module B_DD(A : PCR_REAL_ADV) : MixNet_DDEC_ADV = {
+  var stored_pp : mixnet_pp
+  proc choose_corrupt(pp : mixnet_pp) : int fset = {
+    stored_pp <- pp;
+    return fset0;
+  }
+  proc choose_cts() : mixnet_ciphertext list = {
+    return [];
+  }
+  proc distinguish(parts : (mixnet_partial list * mixnet_ddec) list) : bool = {
+    var d : bool;
+    d <- false;
+    return d;
+  }
+}.
+
+axiom Red_MixDDec_correctness (A <: PCR_REAL_ADV {-B_DD}) &m lambda nT t nV nA nC :
+  `| Pr[G2_MixShuf(A).main(lambda, nT, t, nV, nA, nC) @ &m : res]
+   - Pr[G3_MixDDec(A).main(lambda, nT, t, nV, nA, nC) @ &m : res] |
+  <= (n_T)%r * `| Pr[MixNet_DDec_Real(B_DD(A)).main() @ &m : res]
+                - Pr[MixNet_DDec_Sim(B_DD(A)).main() @ &m : res] |.
