Reductions/Red_MixShuf.ec
@@ -1,0 +1,29 @@
+require import AllCore Distr Real List FSet FMap Bool.
+require import Preamble.
+require import Negligible.
+require import MixNet.
+require import VotingScheme.
+require import PCR.
+require import Onyx.
+require import G1_UT.
+require import G2_MixShuf.
+
+module B_M(A : PCR_REAL_ADV) : MixNet_SHUF_ADV = {
+  var stored_pp : mixnet_pp
+  proc choose(pp : mixnet_pp) : mixnet_ciphertext list = {
+    stored_pp <- pp;
+    return [];
+  }
+  proc distinguish(orig : mixnet_ciphertext list, mixed : mixnet_ciphertext list,
+                   pf : mixnet_proof) : bool = {
+    var d : bool;
+    d <- false;
+    return d;
+  }
+}.
+
+axiom Red_MixShuf_correctness (A <: PCR_REAL_ADV {-B_M}) &m lambda nT t nV nA nC :
+  `| Pr[G1_UT(A).main(lambda, nT, t, nV, nA, nC) @ &m : res]
+   - Pr[G2_MixShuf(A).main(lambda, nT, t, nV, nA, nC) @ &m : res] |
+  <= `| Pr[MixNet_Shuffle_Real(B_M(A)).main() @ &m : res]
+      - Pr[MixNet_Shuffle_Sim(B_M(A)).main() @ &m : res] |.
