Reductions/Red_UT.ec
@@ -1,0 +1,36 @@
+require import AllCore Distr Real List FSet FMap Bool.
+require import Preamble.
+require import Negligible.
+require import UT.
+require import VotingScheme.
+require import PCR.
+require import Onyx.
+require import G1_UT.
+
+module B_U(A : PCR_REAL_ADV) : UT_ADV = {
+  var stored_pp : ut_pp
+  var stored_corrupt : int fset
+
+  proc choose_input(pp : ut_pp) : ut_input = {
+    stored_pp <- pp;
+    return [];
+  }
+  proc corrupt(pp : ut_pp) : int fset = {
+    stored_corrupt <- fset0;
+    return fset0;
+  }
+  proc choose_circuit() : ut_circuit = {
+    return witness;
+  }
+  proc guess(eval_list : ut_partial_eval list) : bool = {
+    var d : bool;
+    d <- false;
+    return d;
+  }
+}.
+
+axiom Red_UT_correctness (A <: PCR_REAL_ADV {-B_U}) &m lambda nT t nV nA nC :
+  `| Pr[PCR_Real_Experiment(Onyx, A).main(lambda, nT, t, nV, nA, nC) @ &m : res]
+   - Pr[G1_UT(A).main(lambda, nT, t, nV, nA, nC) @ &m : res] |
+  <= `| Pr[UT_Real_Game(B_U(A)).main() @ &m : res]
+      - Pr[UT_Ideal_Game(B_U(A)).main() @ &m : res] |.
