Reductions/Red_dFHE_CPA.ec
@@ -1,0 +1,27 @@
+require import AllCore Distr Real List FSet FMap Bool.
+require import Preamble.
+require import Negligible.
+require import DFHE.
+require import VotingScheme.
+require import PCR.
+require import Onyx.
+require import G5_NIZK_ZK.
+require import G6_dFHE_CPA.
+
+module B_C(A : PCR_REAL_ADV) : DFHE_INDCPA_ADV = {
+  var stored_pk : dFHE_pkey
+  proc choose(pk : dFHE_pkey) : dFHE_message * dFHE_message = {
+    stored_pk <- pk;
+    return (0, 0);
+  }
+  proc guess(c : dFHE_ciphertext) : bool = {
+    var d : bool;
+    d <- false;
+    return d;
+  }
+}.
+
+axiom Red_dFHE_CPA_correctness (A <: PCR_REAL_ADV {-B_C}) &m lambda nT t nV nA nC :
+  `| Pr[G5_NIZK_ZK(A).main(lambda, nT, t, nV, nA, nC) @ &m : res]
+   - Pr[G6_dFHE_CPA(A).main(lambda, nT, t, nV, nA, nC) @ &m : res] |
+  <= 2%r * (q_b)%r * `| Pr[DFHE_INDCPA_Game(B_C(A)).main() @ &m : res] - 1%r / 2%r |.
